Eliminate NLustre subdirectories
The decision procedures and properties are now included in the main
file to simplify working with the NLustre files.

NLustre/IsFree.v
@@ -110,6 +110,319 @@ Module Type ISFREE
        Is_free_in_laexp Is_free_in_laexps Is_free_in_cexp
        Is_free_in_caexp Is_free_in_eq.
 
+  (** * Decision procedure *)
+
+  (* TODO: use auto for the proofs. *)
+
+  Lemma Is_free_in_clock_disj:
+    forall y ck x c, Is_free_in_clock y (Con ck x c)
+                     <-> y = x \/ Is_free_in_clock y ck.
+  Proof.
+    intros y ck x c; split; intro HH.
+    inversion_clear HH; [left; reflexivity|right; assumption].
+    destruct HH as [HH|HH].
+    rewrite HH; constructor.
+    constructor (assumption).
+  Qed.
+
+  Lemma Is_free_in_when_disj:
+    forall y e x c, Is_free_in_lexp y (Ewhen e x c)
+                    <-> y = x \/ Is_free_in_lexp y e.
+  Proof.
+    intros y e x c; split; intro HH.
+    inversion_clear HH; auto.
+    destruct HH as [HH|HH].
+    rewrite HH; constructor (fail).
+    constructor (assumption).
+  Qed.
+
+  Fixpoint free_in_clock_dec (ck : clock) (T: PS.t)
+    : { S | forall x, PS.In x S <-> (Is_free_in_clock x ck \/ PS.In x T) }.
+    refine (
+        match ck with
+        | Cbase => exist _ T _
+        | Con ck' x c =>
+          match free_in_clock_dec ck' T with
+          | exist S' HF => exist _ (PS.add x S') _
+          end
+        end).
+    - intro x; split; intro HH.
+      right; exact HH.
+      destruct HH as [HH|HH]; [inversion HH|exact HH].
+    - intro y; split; intro HH.
+      + rewrite PS.add_spec in HH.
+        destruct HH as [HH|HH].
+        rewrite HH; left; constructor.
+        apply HF in HH.
+        destruct HH as [HH|HH]; [left|right].
+        constructor (assumption). assumption.
+      + rewrite Is_free_in_clock_disj in HH.
+        apply or_assoc in HH.
+        destruct HH as [HH|HH].
+        rewrite HH; apply PS.add_spec; left; reflexivity.
+        apply HF in HH; apply PS.add_spec; right; assumption.
+  Defined.
+  
+  Fixpoint free_in_clock (ck : clock) (fvs: PS.t) : PS.t :=
+    match ck with
+    | Cbase => fvs
+    | Con ck' x _ => free_in_clock ck' (PS.add x fvs)
+    end.
+
+  Fixpoint free_in_lexp (e: lexp) (fvs: PS.t) : PS.t :=
+    match e with
+    | Econst _ => fvs
+    | Evar x _ => PS.add x fvs
+    | Ewhen e x _ => free_in_lexp e (PS.add x fvs)
+    | Eunop _ e _ => free_in_lexp e fvs
+    | Ebinop _ e1 e2 _ => free_in_lexp e2 (free_in_lexp e1 fvs)
+    end.
+
+  Definition free_in_laexp (ck: clock)(le : lexp) (fvs : PS.t) : PS.t :=
+    free_in_lexp le (free_in_clock ck fvs).
+
+  Definition free_in_laexps (ck: clock)(les : lexps) (fvs : PS.t) : PS.t :=
+    fold_left (fun fvs e => free_in_lexp e fvs) les (free_in_clock ck fvs).
+
+  Fixpoint free_in_cexp (ce: cexp) (fvs: PS.t) : PS.t :=
+    match ce with
+    | Emerge i t f => free_in_cexp f (free_in_cexp t (PS.add i fvs))
+    | Eite b t f => free_in_cexp f (free_in_cexp t (free_in_lexp b fvs))
+    | Eexp e => free_in_lexp e fvs
+    end.
+
+  Definition free_in_caexp (ck: clock)(ce: cexp) (fvs: PS.t) : PS.t :=
+    free_in_cexp ce (free_in_clock ck fvs).
+
+  Fixpoint free_in_equation (eq: equation) (fvs: PS.t) : PS.t :=
+    match eq with
+    | EqDef _ ck cae    => free_in_caexp ck cae fvs
+    | EqApp _ ck f laes => free_in_laexps ck laes fvs
+    | EqFby _ ck v lae  => free_in_laexp ck lae fvs
+    end.
+
+  (** * Specification lemmas *) 
+
+  Lemma free_in_clock_spec:
+    forall x ck m, PS.In x (free_in_clock ck m)
+                   <-> Is_free_in_clock x ck \/ PS.In x m.
+  Proof.
+    induction ck.
+    - split; intuition;
+        (match goal with H:Is_free_in_clock _ Cbase |- _ => inversion H end).
+    - split; intro H0.
+      + apply IHck in H0; destruct H0 as [H0|H0]; try apply PS.add_spec in H0;
+          intuition; subst; intuition.
+      + apply IHck; destruct H0 as [H0|H0]; inversion H0;
+          solve [right; apply PS.add_spec; intuition | intuition].
+  Qed.
+  
+  Corollary free_in_clock_spec':
+    forall x ck, PS.In x (free_in_clock ck PS.empty)
+                 <-> Is_free_in_clock x ck.
+  Proof.
+    intros; pose proof (free_in_clock_spec x ck PS.empty) as H0;
+      intuition not_In_empty.
+  Qed.
+
+  Lemma free_in_lexp_spec:
+    forall x e m, PS.In x (free_in_lexp e m)
+                  <-> Is_free_in_lexp x e \/ PS.In x m.
+  Proof.
+    intro x; induction e using lexp_ind;
+      try now intro m; (split;
+                        [
+                          intro H0; try apply IHe in H0
+                        | intro H0; try apply IHe
+                       ]);
+      try destruct H0 as [H0|H0];
+      try apply free_in_clock_spec in H0;
+      try inversion H0; subst;
+        try apply PS.add_spec;
+        solve [
+            intuition
+          | right; apply free_in_clock_spec; intuition
+          | apply PS.add_spec in H1; destruct H1; subst; intuition
+          | right; apply PS.add_spec; intuition ].
+    intro m.
+    split; intro HH.
+    - simpl in HH.
+      apply IHe2 in HH.
+      destruct HH as [HH|HH]; [now intuition|].
+      apply IHe1 in HH. intuition.
+    - simpl.
+      destruct HH as [HH|HH].
+      + inversion_clear HH as [| | | |? ? ? ? ? Hf].
+        apply IHe2.
+        destruct Hf as [HH|HH]; intuition.
+        right. apply IHe1; intuition.
+      + apply IHe2; right; apply IHe1; intuition.
+  Qed.          
+
+  Lemma free_in_lexp_spec':
+    forall x e, PS.In x (free_in_lexp e PS.empty)
+                <-> Is_free_in_lexp x e.
+  Proof.
+    intros; pose proof (free_in_lexp_spec x e PS.empty);
+      intuition not_In_empty.
+  Qed.
+
+  Lemma free_in_laexp_spec:
+    forall x ck e m, PS.In x (free_in_laexp ck e m)
+                     <-> Is_free_in_laexp x ck e \/ PS.In x m.
+  Proof.
+    destruct e; split; intros;
+      repeat
+        (match goal with
+         | H:_ \/ _ |- _ => destruct H as [H|H]
+         | H:PS.In _ (free_in_laexp _ _ _) |- _ => apply free_in_lexp_spec in H
+         | H:PS.In _ (free_in_clock _ _) |- _ => apply free_in_clock_spec in H
+         | |- PS.In _ (free_in_laexp _ _ _) => apply free_in_lexp_spec
+         | H:Is_free_in_laexp _ _ _ |- _ => inversion_clear H
+         | |- context[PS.In _ (free_in_clock _ _)] => rewrite free_in_clock_spec
+         end);
+      intuition.
+  Qed.
+
+  Lemma free_in_laexp_spec':
+    forall x ck e, PS.In x (free_in_laexp ck e PS.empty)
+                   <-> Is_free_in_laexp x ck e.
+  Proof.
+    intros; pose proof (free_in_laexp_spec x ck e PS.empty);
+      intuition not_In_empty.
+  Qed.
+
+  Lemma free_in_fold_left_lexp_spec : forall x l m,
+      PS.In x (fold_left (fun fvs e => free_in_lexp e fvs) l m) <->
+      Exists (Is_free_in_lexp x) l \/ PS.In x m.
+  Proof.
+    Local Hint Constructors Exists.
+    intros x l. induction l; intro m; simpl.
+    - intuition.
+      match goal with H:Exists _ nil |- _ => inversion H end.
+    - rewrite IHl. rewrite free_in_lexp_spec.
+      split; intros [H | H]; auto.
+      + destruct H as [H | H]; auto.
+      + inversion_clear H; auto.
+  Qed.
+
+  Lemma free_in_laexps_spec:
+    forall x ck e m, PS.In x (free_in_laexps ck e m)
+                     <-> Is_free_in_laexps x ck e \/ PS.In x m.
+  Proof.
+    intros x c l m. unfold free_in_laexps.
+    rewrite free_in_fold_left_lexp_spec.
+    rewrite free_in_clock_spec.
+    split; intros [H | H]; auto; inversion H; auto.
+  Qed.
+
+  Lemma free_in_laexps_spec':
+    forall x ck l, PS.In x (free_in_laexps ck l PS.empty)
+                   <-> Is_free_in_laexps x ck l.
+  Proof.
+    intros; pose proof (free_in_laexps_spec x ck l PS.empty);
+      intuition not_In_empty.
+  Qed.
+
+  Ltac destruct_Is_free :=
+    repeat match goal with
+           | H: _ \/ _ |- _ =>
+             destruct H
+
+           | H: Is_free_in_cexp _ (Emerge _ _ _) |- _ =>
+             inversion H; subst; clear H
+
+           | H: Is_free_in_cexp _ (Eexp _) |- _ =>
+             inversion H; subst; clear H
+
+           | IHe: context[PS.In _ (free_in_cexp ?e _)],
+                  H:PS.In _ (free_in_cexp ?e _) |- _ =>
+             apply IHe in H
+
+           | H: PS.In _ (free_in_lexp _ _) |- _ =>
+             apply free_in_lexp_spec in H
+
+           | H: PS.In _ (PS.add _ _) |- _ =>
+             apply PS.add_spec in H
+           end.
+
+  Lemma free_in_cexp_spec:
+    forall x e m, PS.In x (free_in_cexp e m)
+                  <-> Is_free_in_cexp x e \/ PS.In x m.
+  Proof.
+    intro x;
+      induction e;
+      intro m; simpl; split; intro H0;
+        destruct_Is_free;
+        subst; auto;
+          try rewrite IHe2, IHe1;
+          try rewrite free_in_lexp_spec;
+          match goal with
+          | H:Is_free_in_cexp _ _ |- _ => inversion_clear H
+          | |- _ => idtac
+          end;
+          intuition.
+  Qed.
+
+  Lemma free_in_cexp_spec':
+    forall x e, PS.In x (free_in_cexp e PS.empty)
+                <-> Is_free_in_cexp x e.
+  Proof.
+    intros; pose proof (free_in_cexp_spec x e PS.empty);
+      intuition not_In_empty.
+  Qed.
+
+  Lemma free_in_caexp_spec:
+    forall x ck e m, PS.In x (free_in_caexp ck e m)
+                     <-> Is_free_in_caexp x ck e \/ PS.In x m.
+  Proof.
+    destruct e; split; intros;
+      repeat progress (match goal with
+           | H:_ \/ _ |- _ => destruct H as [H|H]
+           | H:PS.In _ _ |- _ => first [ apply free_in_cexp_spec in H
+                                       | apply free_in_clock_spec in H ]
+           | |- context [free_in_caexp _ _ _] => apply free_in_cexp_spec
+           | H:Is_free_in_caexp _ _ _ |- _ => inversion_clear H
+           | _ => solve [right; apply free_in_clock_spec; intuition
+                        | intuition]
+                       end).
+  Qed.
+  
+  Lemma free_in_caexp_spec':
+    forall x ck e, PS.In x (free_in_caexp ck e PS.empty)
+                   <-> Is_free_in_caexp x ck e.
+  Proof.
+    intros; rewrite (free_in_caexp_spec x ck e PS.empty).
+    intuition not_In_empty.
+  Qed.
+
+  Lemma free_in_equation_spec:
+    forall x eq m, PS.In x (free_in_equation eq m)
+                   <-> (Is_free_in_eq x eq \/ PS.In x m).
+  Proof.
+    destruct eq; split; intro H;
+      repeat (match goal with
+              | H:Is_free_in_eq _ _ |- _ => inversion_clear H
+              | H:PS.In _ (free_in_equation _ _) |- _ =>
+                apply free_in_caexp_spec in H
+                || apply free_in_laexp_spec in H
+                || apply free_in_laexps_spec in H
+              | |- PS.In _ (free_in_equation _ _) =>
+                apply free_in_caexp_spec
+                || apply free_in_laexp_spec
+                || apply free_in_laexps_spec
+              | _ => intuition
+              end).
+  Qed.
+
+  Lemma free_in_equation_spec':
+    forall x eq, PS.In x (free_in_equation eq PS.empty)
+               <-> Is_free_in_eq x eq.
+  Proof.
+    intros; rewrite (free_in_equation_spec x eq PS.empty).
+    intuition not_In_empty.
+  Qed.
+
 End ISFREE.
 
 Module IsFreeFun
