NLustre.v
@@ -15,11 +15,6 @@ Require Export NLustre.Clocking.
 Require Export NLustre.NLTyping.
 
 Require Import Velus.Common.
-Require Import NLustre.IsVariable.Decide.
-Require Import NLustre.IsDefined.Decide.
-Require Import NLustre.WellFormed.Decide.
-Require Import NLustre.IsFree.Decide.
-Require Export NLustre.Clocking.Properties.
 
 Module Type NLUSTRE
        (Ids   : IDS)
@@ -30,7 +25,6 @@ Module Type NLUSTRE
   Declare Module Export Str: STREAM Op.
   Declare Module Export Ord: ORDERED Ids Op Clks Syn.
   Declare Module Export IsF: ISFREE Ids Op Clks Syn.
-  Declare Module Export IsFDec: IsFree.Decide.DECIDE Ids Op Clks Syn IsF.
   Declare Module Export Sem: NLSEMANTICS Ids Op OpAux Clks Syn Str Ord.
   Declare Module Export Typ: NLTYPING Ids Op Clks Syn.
   Declare Module Export Mem: MEMORIES Ids Op Clks Syn.
@@ -40,12 +34,7 @@ Module Type NLUSTRE
   Declare Module Export WeF: WELLFORMED Ids Op Clks Syn IsF Ord Mem IsD IsV NoD.
   Declare Module Export MemSem: MEMSEMANTICS Ids Op OpAux Clks Syn Str Ord Mem
                                     IsF IsD Sem IsV NoD WeF.     
-  Declare Module Export IsVDec: IsVariable.Decide.DECIDE Ids Op Clks Syn Mem IsD IsV.
-  Declare Module Export IsDDec: IsDefined.Decide.DECIDE Ids Op Clks Syn Mem IsD.
-  Declare Module Export IsWFDec: WellFormed.Decide.DECIDE Ids Op Clks Syn IsF IsFDec
-                                     Ord Mem IsD IsV IsDDec IsVDec NoD WeF.
-  Declare Module Export Clo: CLOCKING Ids Op Clks Syn.
-  Declare Module Export Pro: PROPERTIES Ids Op Clks Syn IsF Clo Mem IsD.
+  Declare Module Export Clo: CLOCKING Ids Op Clks Syn IsF Mem IsD.
 End NLUSTRE.
 
 Module NLustreFun
@@ -58,7 +47,6 @@ Module NLustreFun
   Module Export Str := StreamFun          Op.
   Module Export Ord := OrderedFun     Ids Op Clks Syn.
   Module Export IsF := IsFreeFun      Ids Op Clks Syn.
-  Module Export IsFDec := IsFree.Decide.DecideFun Ids Op Clks Syn IsF.
   Module Export Sem := NLSemanticsFun Ids Op OpAux Clks Syn Str Ord.
   Module Export Typ := NLTypingFun    Ids Op Clks Syn.
   Module Export Mem := MemoriesFun    Ids Op Clks Syn.
@@ -68,11 +56,6 @@ Module NLustreFun
   Module Export WeF := WellFormedFun  Ids Op Clks Syn IsF Ord Mem IsD IsV NoD.
   Module Export MemSem := MemSemanticsFun Ids Op OpAux Clks Syn Str Ord Mem IsF
                             IsD Sem IsV NoD WeF.     
-  Module Export IsVDec := IsVariable.Decide.DecideFun Ids Op Clks Syn Mem IsD IsV.
-  Module Export IsDDec := IsDefined.Decide.DecideFun Ids Op Clks Syn Mem IsD.
-  Module Export IsWFDec := WellFormed.Decide.DecideFun Ids Op Clks Syn IsF
-                            IsFDec Ord Mem IsD IsV IsDDec IsVDec NoD WeF.
-  Module Export Clo := ClockingFun    Ids Op Clks Syn.
-  Module Export Pro := PropertiesFun  Ids Op Clks Syn IsF Clo Mem IsD.
+  Module Export Clo := ClockingFun    Ids Op Clks Syn IsF Mem IsD.
 End NLustreFun.
 
